SEAR/SEARappend.sml
@@ -1,0 +1,165 @@
+val Listn_def =
+    Thm_2_4' |> qtinst_thm [(‘A’,‘List(A)’)]
+             |> qfVar_prpl_th1 
+             ("P",[‘l:mem(List(A))’],
+              ‘Length(l:mem(List(A))) = n’)     
+             |> set_spec (rastt "List(A)") "Listn" "iLn" [("A",set_sort),("n",mem_sort (rastt "N"))]
+             |> gen_all
+
+
+(*1.can pick a base point, and use inverse *)
+(*2.can directly prove unique existence, since existence of list items implies existence of term*)
+
+val RepLn_def = qdefine_fsym ("RepLn",[‘ln:mem(Listn(A,n:mem(N)))’])
+                            ‘App(iLn(A,n),ln)’
+                            |> gen_all |> store_as "RepLn_def";
+
+
+
+
+val LnNil_def = proved_th $
+e0
+(strip_tac >> uex_tac >>
+ qspecl_then [‘A’] strip_assume_tac Listn_def >>
+ first_assum (qspecl_then [‘O’] strip_assume_tac) >>
+ first_assum (qspecl_then [‘Nil(A)’] assume_tac) >>
+ fs[Length_Nil] >>
+ qexists_tac ‘b’ >> arw[RepLn_def] >>
+ fs[Inj_def])
+(form_goal “!A. ?!ln:mem(Listn(A,O)).RepLn(ln) = Nil(A)”)
+|> spec_all |> qsimple_uex_spec "LnNil" [‘A’] |> gen_all
+|> store_as "LnNil_def";
+
+
+
+(*
+val om0_def = qfun_compr ‘f:mem(Exp(A,B))’ ‘Tpm((f0:B->C) o tof(f))’
+                               |>  qsimple_uex_spec "om0" [‘f0’,‘A’] |> gen_all
+*)
+
+
+val CONSe_def =  qfun_compr ‘l:mem(List(A))’ ‘Cons(a,l)’
+                               |>  qsimple_uex_spec "CONSe" [‘a:mem(A)’] |> gen_all
+
+val aprecf_def = 
+qfun_compr ‘af:mem(A * Exp(List(A),List(A)))’ 
+‘Tpm(CONSe(Fst(af)) o tof(Snd(af)))’
+|> qsimple_uex_spec "aprecf" [‘A’] |> gen_all
+
+
+val APPEND0_def = qdefine_fsym ("APPEND0",[‘A’]) ‘Lrec(Tpm(Id(List(A))),aprecf(A))’ |> gen_all
+
+val Append_def = 
+qdefine_fsym ("Append",[‘l1:mem(List(A))’,‘l2:mem(List(A))’])
+                            ‘App(tof(App(APPEND0(A),l1)),l2)’
+                            |> gen_all |> store_as "Append_def";
+
+
+val Length_RepLn = proved_th $
+e0
+(rpt strip_tac >>
+ qspecl_then [‘A’,‘n’,‘l’] assume_tac RepLn_def >>
+ arw[] >>
+ qspecl_then [‘A’,‘n’] strip_assume_tac Listn_def >>
+ arw[] >> qexists_tac ‘l’ >> rw[])
+(form_goal “!A n l:mem(Listn(A,n)). Length(RepLn(l)) = n”)
+
+val RepLn_Listn_LENGTH_eq = proved_th $
+e0
+(rpt strip_tac >> 
+ qby_tac ‘Length(RepLn(l1)) =Length(RepLn(l2))’  
+ >-- arw[] >>
+ fs[Length_RepLn])
+(form_goal “!A n1 n2 l1:mem(Listn(A,n1)) l2:mem(Listn(A,n2)). RepLn(l1) = RepLn(l2) ==> n1 = n2”)
+
+val APPEND_def = 
+    qfun_compr ‘l1l2:mem(List(A) * List(A))’
+                        ‘Append(Fst(l1l2),Snd(l1l2))’ 
+     |> qsimple_uex_spec "APPEND" [‘l1l2 :mem(List(A) * List(A))’,‘A’]
+     |> gen_all
+
+
+val APPEND0_Nil = proved_th $
+e0
+(rw[APPEND0_def,Lrec_Nil])
+(form_goal “App(APPEND0(A),Nil(A)) = Tpm(Id(List(A)))”)
+
+
+val APPEND0_Cons = proved_th $
+e0
+(rw[APPEND0_def,Lrec_Cons,aprecf_def,Pair_def'])
+(form_goal “App(APPEND0(A),Cons(h,t)) = 
+ Tpm(CONSe(h) o tof(App(APPEND0(A),t)))”)
+
+
+
+val Append_Nil = proved_th $
+e0
+(rw[Append_def,APPEND0_Nil,tof_Tpm_inv,App_Id])
+(form_goal “Append(Nil(X),l) = l”)
+
+val Append_Cons = proved_th $
+e0
+(rw[Append_def,APPEND0_Cons,tof_Tpm_inv,App_App_o,CONSe_def])
+(form_goal “Append(Cons(h:mem(X),t),l) = Cons(h, Append(t,l))”)
+
+
+
+
+(*ind_with need name to be X, lame...*)
+val Length_Append = proved_th $
+e0
+(ind_with List_induct >> rpt strip_tac (* 2 *)
+ >-- (rw[Length_Nil,Add_O2,Append_Nil]) >>
+ arw[Append_Cons,Length_Cons,Add_Suc1]
+ )
+(form_goal
+ “!l1:mem(List(X)) l2. Length(Append(l1,l2)) = Add(Length(l1),Length(l2))”)
+
+val RepLn_eq_eq = proved_th $
+e0
+(rpt strip_tac >>
+  qspecl_then [‘A’,‘n’] strip_assume_tac Listn_def >> 
+  fs[Inj_def,RepLn_def] >>
+  first_assum irule >> arw[])
+(form_goal “!A n l1:mem(Listn(A,n)) l2. RepLn(l1) = RepLn(l2) ==> l1 = l2”)
+
+
+
+val Appendn_ex = proved_th $
+e0
+(rpt strip_tac >>
+ uex_tac >>
+ qspecl_then [‘A’,‘Add(n1,n2)’] strip_assume_tac Listn_def >>
+ first_x_assum $ qspecl_then [‘Append(RepLn(l1),RepLn(l2))’] assume_tac >>
+ fs[Length_Append,Length_RepLn] >>
+ qexists_tac ‘b’ >> rw[RepLn_def] >>
+ rpt strip_tac >>
+ irule RepLn_eq_eq >> arw[RepLn_def])
+(form_goal 
+“!A n1:mem(N) l1:mem(Listn(A,n1)) n2:mem(N) l2:mem(Listn(A,n2)). 
+?!l1l2:mem(Listn(A, Add(n1,n2))). 
+ Append(RepLn(l1),RepLn(l2)) = RepLn(l1l2)”)
+
+
+val Appendn_def = 
+Appendn_ex
+|> spec_all
+|> qsimple_uex_spec "Appendn" [‘l1’,‘l2’] |> gen_all
+
+
+(*
+val Lnabs_def = 
+Abs maps a list to Listn(A,Length(l)).
+
+
+
+val Length_Cons = prove_store("Length_Cons",
+e0
+(rw[Length_def,LENGTH_def,Lrec_Cons,App_App_o,p12_of_Pair,
+    Suc_def])
+(form_goal
+“!A l1:mem(Listn(A,n)) l2:mem(Listn(A,m)). 
+ ?!l12:mem(Listn(A,n+m)). RepLn(l1) 
+ Abs”));
+*)
